dev/lf/tight-proof/Canonical_forms1.v
@@ -22,8 +22,8 @@ Lemma canonical_forms_1: forall G s x T U,
 Proof.
   introv Hwf Hty.
   pose proof (wf_good Hwf) as Hgd.
-  pose proof (general_to_tight_typing Hwf Hty) as Hti.
-  pose proof (tight_to_precise_typ_all Hwf Hti) as [S' [T' [Hpt [Hsub [HSsub [L' HTsub]]]]]].
+  pose proof (general_to_tight_typing Hgd Hty) as Hti.
+  pose proof (tight_to_precise_typ_all Hgd Hti) as [S' [T' [Hpt [Hsub [HSsub [L' HTsub]]]]]].
   pose proof (good_precise_all_inv Hgd Hpt) as Bi.
   pose proof (corresponding_types Hwf Bi) as [[T2 [U2 [t [Hb [Hl HS]]]]] | [? [? [? [? HS]]]]];
   inversion HS.
