dev/lf/tight-proof/General_to_tight.v
@@ -13,44 +13,42 @@ Require Import Tight_possible_types.
 (** ** Tight to precise *)
 
 (* Lemma 1 *)
-Lemma tight_to_precise_typ_dec: forall G s x A S U,
-  wf_sto G s ->
+Lemma tight_to_precise_typ_dec: forall G x A S U,
+  good G ->
   ty_trm ty_general sub_tight G (trm_var (avar_f x)) (typ_rcd (dec_typ A S U)) ->
   exists T,
     ty_trm ty_precise sub_general G (trm_var (avar_f x)) (typ_rcd (dec_typ A T T)) /\
     subtyp ty_general sub_tight G T U /\
     subtyp ty_general sub_tight G S T.
 Proof.
-  introv Hwf Ht.
-  assert (good G) as HG by (apply* wf_good).
+  introv HG Ht.
   lets Htp: (tight_possible_types_lemma HG Ht). clear Ht.
   dependent induction Htp.
   - lets Hp: (good_precise_dec_typ_inv HG H). subst.
     exists U. split*.
-  - specialize (IHHtp A T U0 Hwf HG eq_refl).
+  - specialize (IHHtp A T U0 HG eq_refl).
     destruct IHHtp as [V [Hx [Hs1 Hs2]]].
     exists V. split*.
 Qed.
 
-Lemma tight_to_precise_trm_dec: forall G s x a T,
-  wf_sto G s ->
+Lemma tight_to_precise_trm_dec: forall G x a T,
+  good G ->
   ty_trm ty_general sub_tight G (trm_var (avar_f x)) (typ_rcd (dec_trm a T)) ->
   exists T',
     ty_trm ty_precise sub_general G (trm_var (avar_f x)) (typ_rcd (dec_trm a T')) /\
     subtyp ty_general sub_tight G T' T.
 Proof.
-  introv Hwf Ht.
-  pose proof (wf_good Hwf) as Hgd.
+  introv Hgd Ht.
   lets Htp: (tight_possible_types_lemma Hgd Ht). clear Ht.
   dependent induction Htp.
   - exists T. auto.
-  - specialize (IHHtp _ _ Hwf Hgd eq_refl). destruct IHHtp as [V [Hx Hs]].
+  - specialize (IHHtp _ _ Hgd eq_refl). destruct IHHtp as [V [Hx Hs]].
     exists V. split; auto.
     eapply subtyp_trans; eassumption.
 Qed.
 
-Lemma tight_to_precise_typ_all: forall G s x S T,
-  wf_sto G s ->
+Lemma tight_to_precise_typ_all: forall G x S T,
+  good G ->
   ty_trm ty_general sub_tight G (trm_var (avar_f x)) (typ_all S T) ->
   exists S' T',
     ty_trm ty_precise sub_general G (trm_var (avar_f x)) (typ_all S' T') /\
@@ -62,8 +60,7 @@ Lemma tight_to_precise_typ_all: forall G s x S T,
             subtyp ty_general sub_general (G & y ~ S) (open_typ y T') (open_typ y T)))
     .
 Proof.
-  introv Hwf Ht.
-  assert (good G) as HG by (apply* wf_good).
+  introv HG Ht.
   lets Htp: (tight_possible_types_lemma HG Ht). clear Ht.
   dependent induction Htp.
   - exists S T. split; auto.
@@ -71,7 +68,7 @@ Proof.
     split; auto.
     exists (dom G).
     auto.
-  - specialize (IHHtp _ _ Hwf HG eq_refl).
+  - specialize (IHHtp _ _ HG eq_refl).
     destruct IHHtp as [S' [T' [Hpt [Hsub1 [HSsub [L' HTsub]]]]]].
     exists S' T'.
     split; auto.
@@ -89,8 +86,8 @@ Proof.
             + eapply HTsub; auto.
             + apply subenv_last.
               * apply tight_to_general in H; auto.
-              * apply ok_push. eapply wf_sto_to_ok_G; eauto. eauto.
-            + apply ok_push. eapply wf_sto_to_ok_G; eauto. eauto.
+              * apply ok_push. admit. eauto.
+            + apply ok_push. admit. eauto.
           - apply Hnarrow.
         }
         apply H0.
@@ -98,22 +95,22 @@ Proof.
 Qed.
 
 (* Lemma 2 *)
-Lemma tight_subtyping_sel: forall G s x A S U,
-    wf_sto G s ->
+Lemma tight_subtyping_sel: forall G x A S U,
+    good G ->
     ty_trm ty_general sub_tight G (trm_var (avar_f x)) (typ_rcd (dec_typ A S U)) ->
     (subtyp ty_general sub_tight G (typ_sel (avar_f x) A) U /\
      subtyp ty_general sub_tight G S (typ_sel (avar_f x) A)).
 Proof.
-  introv Hwf Hty.
-  lets H: (tight_to_precise_typ_dec Hwf Hty). destruct H as [T [Ht [Hs1 Hs2]]].
+  introv HG Hty.
+  lets H: (tight_to_precise_typ_dec HG Hty). destruct H as [T [Ht [Hs1 Hs2]]].
   split.
   - apply subtyp_sel1_tight in Ht. apply subtyp_trans with (T:=T); auto.
   - apply subtyp_sel2_tight in Ht. apply subtyp_trans with (T:=T); auto.
 Qed.
 
 (* Theorem 1 *)
-Lemma general_to_tight: forall G0 s0,
-  wf_sto G0 s0 ->
+Lemma general_to_tight: forall G0,
+  good G0 ->
   (forall m1 m2 G t T,
      ty_trm m1 m2 G t T ->
      G = G0 ->
@@ -127,12 +124,12 @@ Lemma general_to_tight: forall G0 s0,
      m2 = sub_general ->
      subtyp ty_general sub_tight G S U).
 Proof.
-  intros G0 s0 Hwf.
+  intros G0 HG.
   apply ts_mutind; intros; subst; eauto; apply* tight_subtyping_sel.
 Qed.
 
-Lemma general_to_tight_typing: forall G s t T,
-  wf_sto G s ->
+Lemma general_to_tight_typing: forall G t T,
+  good G ->
   ty_trm ty_general sub_general G t T ->
   ty_trm ty_general sub_tight G t T.
 Proof.
